src/Ast/Resolver.dfy
@@ -10,31 +10,53 @@ module Resolver {
   import opened Ast
 
   method Resolve(b3: Raw.Program) returns (r: Result<Ast.Program, string>)
-    ensures r.Success? ==> b3.WellFormed()
+    ensures r.Success? ==> b3.WellFormed() && r.value.WellFormed()
   {
     var boolType := new Type(BoolTypeName);
     var intType := new Type(IntTypeName);
     var typeMap := map[BoolTypeName := boolType, IntTypeName := intType];
     for n := 0 to |b3.types|
-      invariant BuiltInTypes <= typeMap.Keys
-      invariant forall i :: 0 <= i < n ==> b3.types[i] in typeMap.Keys && b3.types[i] !in BuiltInTypes
+      // invariants about typeMap
+      invariant typeMap.Keys == BuiltInTypes + set typename <- b3.types[..n]
       invariant MapIsInjective(typeMap)
+      // invariants related to showing we've checked the conditions of RawAst well-formedness
+      invariant forall typename <- b3.types[..n] :: typename !in BuiltInTypes
       invariant forall i, j :: 0 <= i < j < n ==> b3.types[i] != b3.types[j]
+      // invariants related to showing that the resolved declarations are well-formed
+      invariant BuiltInTypes <= (set typ: Type <- typeMap.Values :: typ.Name)
+      invariant forall typename <- typeMap.Keys :: typeMap[typename].Name == typename
     {
-      var typename := b3.types[n];
-      if typename in typeMap.Keys {
-        return Failure("duplicate type name: " + typename);
+      var name := b3.types[n];
+      if name in typeMap.Keys {
+        return Failure("duplicate type name: " + name);
       }
-      var typ := new Type(typename);
-      typeMap := typeMap[typename := typ];
-    }
-    assert forall typ <- b3.types :: typ !in BuiltInTypes;
-    assert forall i, j :: 0 <= i < j < |b3.types| ==> b3.types[i] != b3.types[j];
-
-    if |b3.procedures| == 0 { // TODO
-      return Success(Program(typeMap.Values, {}));
+      var typ := new Type(name);
+      typeMap := typeMap[name := typ];
     }
 
-    return Failure("good so far, but resolver is not yet fully implemented");
+    var procMap: map<string, Procedure> := map[];
+    for n := 0 to |b3.procedures|
+      // invariants about procMap
+      invariant procMap.Keys == set proc <- b3.procedures[..n] :: proc.name
+      invariant MapIsInjective(procMap)
+      // invariants related to showing we've checked the conditions of RawAst well-formedness
+      invariant forall i, j :: 0 <= i < j < n ==> b3.procedures[i].name != b3.procedures[j].name
+      invariant forall proc <- b3.procedures[..n] :: proc.WellFormed(b3)
+      // invariants related to showing that the resolved declarations are well-formed
+      invariant forall procname <- procMap.Keys :: procMap[procname].Name == procname
+    {
+      var proc := b3.procedures[n];
+      var name := proc.name;
+      if name in procMap.Keys {
+        return Failure("duplicate procedure name: " + name);
+      }
+      var rproc := new Procedure(name, [], Nil, Nil); // TODO: other parameters
+      procMap := procMap[name := rproc];
+      assume {:axiom} proc.WellFormed(b3); // TODO
+    }
+
+    var r3 := Program(typeMap.Values, procMap.Values);
+
+    return Success(r3);
   }
 }
