src/RawAst/RawAst.dfy
@@ -11,8 +11,8 @@ module RawAst {
     predicate WellFormed() {
       && (forall typ <- types :: typ !in BuiltInTypes)
       && (forall i, j :: 0 <= i < j < |types| ==> types[i] != types[j])
-      && (forall proc <- procedures, proc' <- procedures :: proc.name == proc'.name ==> proc == proc')
-      && forall proc <- procedures :: proc.WellFormed(this)
+      && (forall i, j :: 0 <= i < j < |procedures| ==> procedures[i].name != procedures[j].name)
+      && (forall proc <- procedures :: proc.WellFormed(this))
     }
 
     method FindProcedure(name: string) returns (r: Option<Procedure>) {
